thir-elab/lib/ast_utils.ml
@@ -105,12 +105,16 @@ module Make (F : Features.T) = struct
           expr e
       end
 
-    let rename_global_idents (f : global_ident -> global_ident) =
+    type level = ExprLevel | TypeLevel
+
+    let rename_global_idents (f : level -> global_ident -> global_ident) =
       object
         inherit [_] item_map as super
-        method visit_t () x = x
-        method visit_mutability _ () m = m
-        method! visit_global_ident s ident = f ident
+        method visit_t (lvl : level) x = x
+        method visit_mutability _ (lvl : level) m = m
+        method! visit_global_ident (lvl : level) ident = f lvl ident
+        method! visit_ty _ t = super#visit_ty TypeLevel t
+        (* method visit_GlobalVar (lvl : level) i = GlobalVar (f lvl i) *)
       end
   end
 
@@ -200,6 +204,8 @@ module Make (F : Features.T) = struct
     match t with
     | TApp { ident = `TupleType 1; args = [ GType t ] } -> remove_tuple1 t
     | _ -> t
+
+  (* let rec remove_empty_tap *)
 
   let is_unit_typ : ty -> bool =
     remove_tuple1 >> [%matches? TApp { ident = `TupleType 0 }]
