thir-elab/lib/desugar_legacy_hacspec_lib.ml
@@ -1,0 +1,89 @@
+open Base
+open Utils
+
+module%inlined_contents Make (FA : Features.T) = struct
+  open Ast
+
+  module FB = struct
+    include FA
+    include Features.Off.Macro
+  end
+
+  module A = Ast.Make (FA)
+  module B = Ast.Make (FB)
+
+  module S = struct
+    include Features.SUBTYPE.Id
+
+    let macro _ = failwith "macro in expression"
+  end
+
+  let metadata = Desugar_utils.Metadata.make "desugar_legacy_hacspec_lib"
+
+  module UA = Ast_utils.Make (FA)
+  module UB = Ast_utils.Make (FB)
+
+  [%%inline_defs "*" - ditem - ditem']
+
+  let ns_gident (n : string * string list) (last_chunk : string) : global_ident
+      =
+    let path = Non_empty_list.of_list_exn (snd n @ [ last_chunk ]) in
+    `Concrete { crate = fst n; path }
+
+  let empty_generics = B.{ params = []; constraints = [] }
+
+  let hacspec_lib_item s =
+    `Concrete { crate = "hacspec"; path = Non_empty_list.[ "lib"; s ] }
+
+  let mk_ty_alias ~name ty = B.TyAlias { name; generics = empty_generics; ty }
+
+  let mk_tapp ~name args =
+    B.TApp
+      {
+        ident = hacspec_lib_item name;
+        args = List.map ~f:(fun x -> B.GType x) args;
+      }
+
+  let mk_ty_name ~name = mk_tapp ~name []
+
+  let rec ditem (item : A.item) : B.item list =
+    match item.v with
+    | [%inline_arms "ditem'.*"] ->
+        map (fun v ->
+            [
+              B.
+                {
+                  v;
+                  span = item.span;
+                  parent_namespace = item.parent_namespace;
+                };
+            ])
+  (* | IMacroInvokation { macro = `Concrete c; argument; span } -> *)
+  (*     failwith @@ [%show: concrete_ident] c *)
+  (* | IMacroInvokation *)
+  (*     { *)
+  (*       macro = *)
+  (*         `Concrete *)
+  (*           Non_empty_list. *)
+  (*             { crate = "hacspec_lib"; path = [ "array"; "array" ] }; *)
+  (*       argument; *)
+  (*       span; *)
+  (*     } -> *)
+  (*     let open Hacspeclib_macro_parser in *)
+  (*     let o : Array.t = Array.parse argument |> Result.ok_or_failwith in *)
+  (*     [ *)
+  (*       B. *)
+  (*         { *)
+  (*           parent_namespace = item.parent_namespace; *)
+  (*           span = item.span; *)
+  (*           v = *)
+  (*             mk_ty_alias ~name:(ns_gident item.parent_namespace o.array_name) *)
+  (*             @@ mk_tapp "lseq" *)
+  (*                  [ mk_ty_name o.typ; mk_ty_name (string_of_int o.size) ]; *)
+  (*         }; *)
+  (*     ] *)
+  (* | IMacroInvokation _ -> [] *)
+
+  module FA = FA
+end
+[@@add "subtype.ml"]
