thir-elab/lib/import_thir.ml
@@ -635,6 +635,13 @@ module Exn = struct
               body = c_expr body;
               params = [];
             }
+      | TyAlias (ty, generics) ->
+          TyAlias
+            {
+              name = def_id (Option.value_exn item.def_id);
+              generics = c_generics generics;
+              ty = c_ty ty;
+            }
       | Fn (generics, { body; header; params; ret; sig_span }) ->
           Fn
             {
@@ -680,6 +687,14 @@ module Exn = struct
           in
           let variants = [ v ] in
           Type { name; generics; variants; record }
+      | MacroInvokation { macro_ident; argument; span } ->
+          IMacroInvokation
+            {
+              macro = def_id macro_ident;
+              argument;
+              span = c_span span;
+              witness = ();
+            }
       | _ -> NotImplementedYet
     in
     { span; v; parent_namespace = namespace_of_def_id item.owner_id }
