thir-elab/lib/options.ml
@@ -1,0 +1,27 @@
+open Base
+open Utils
+open Ast
+open Cmdliner
+
+(* let count = *)
+(*   let doc = "Repeat the message $(docv) times." in *)
+(*   Arg.(value & opt int 10 & info [ "c"; "count" ] ~docv:"COUNT" ~doc) *)
+
+(* let chorus_t = Term.(const Fn.id $ count) *)
+
+(* let global_ident_cmdliner_converter = *)
+(*   (, fun fmt t -> Format.fprintf fmt "%s" (to_string t)) *)
+
+type t = {
+  output_directory : string;
+  name_remapping : (GlobalIdent.t * GlobalIdent.t) list;
+  binary_operators : (GlobalIdent.t * string) list;
+}
+[@@deriving cmdliner, show]
+
+let main () =
+  let f p = show p |> print_endline in
+  let info = Cmdliner.Cmd.info Sys.argv.(0) in
+  let term = Cmdliner.Term.(const f $ cmdliner_term ()) in
+  let cmd = Cmdliner.Cmd.v info term in
+  exit (Cmdliner.Cmd.eval cmd)
