thir-elab/out/Hacspec_chacha20.Header.old.fst
@@ -3,45 +3,41 @@ module Hacspec_chacha20.Header
 open FStar.Mul
 open Hacspec.Lib
 
-unfold type state_t = lseq uint32 16
-unfold type state_idx = nat_mod 16
+type state_t = lseq (uint32) (16)
 
-unfold type constants_t = lseq uint32 4
-unfold type constants_idx = nat_mod 4
+let state_idx =
+  nat_mod (16)
 
-unfold type block_t = lseq uint8 64
-unfold type chaChaIV_t = lseq uint8 12
-unfold type chaChaKey_t = lseq uint8 32
+type constants_t = lseq (uint32) (4)
 
-class from_seq_tc (t: Type) 
-  = { inner: Type
-    ; size: nat
-    ; from_seq: s:seq inner{seq_len s = size} -> t }
-class array_assign (o: Type0) 
-  = { key: Type0
-    ; value: Type0
-    ; (.[]<-): o -> key -> value -> o }
-class has_new_ (o: Type) = {new_: o}
+let constants_idx =
+  nat_mod (4)
 
-instance from_seq_lseq inner size: from_seq_tc (lseq inner size) 
-  = { inner; size
-    ; from_seq = array_from_seq size }
-    
-instance array_lseq value (s: uint_size {s > 0}): array_assign (lseq value s)
-  = { value; key = nat_mod s
-    ; (.[]<-) = array_upd }
+type block_t = lseq (uint8) (64)
 
-instance has_new_uint64: has_new_ uint64 = {new_ = secret (pub_u64 0)}
-instance has_new_uint32: has_new_ uint32 = {new_ = secret (pub_u32 0)}b
-instance has_new_uint16: has_new_ uint16 = {new_ = secret (pub_u16 0)}
-instance has_new_uint8: has_new_ uint8 = {new_ = secret (pub_u8 0)}
-instance has_new_int64: has_new_ int64 = {new_ = secret (pub_i64 0)}
-instance has_new_int32: has_new_ int32 = {new_ = secret (pub_i32 0)}
-instance has_new_int16: has_new_ int16 = {new_ = secret (pub_i16 0)}
-instance has_new_int8: has_new_ int8 = {new_ = secret (pub_i8 0)}
+type chaChaIV_t = lseq (uint8) (12)
 
-instance has_new_lseq {| has_new_ 'a |} s: has_new_ (lseq 'a s) 
-  = {new_ = array_new_ new_ s}
+type chaChaKey_t = lseq (uint8) (32)
+
+let x = 3l
+
+class from_seq_tc (t: Type) = {
+  inner: Type;
+  size: nat;
+  from_seq: s:seq inner{seq_len s = size} -> t
+}
+
+instance _: from_seq_tc state_t = {
+  inner = uint32;
+  size = 16;
+  from_seq = array_from_seq 16
+}
+
+instance _: from_seq_tc block_t = {
+  inner = uint8;
+  size = 64;
+  from_seq = array_from_seq 64
+}
 
 let to_le_bytes (#int_ty: inttype{unsigned int_ty /\ int_ty <> U1})
   (#len: uint_size{
@@ -51,6 +47,27 @@ let to_le_bytes (#int_ty: inttype{unsigned int_ty /\ int_ty <> U1})
 
 let to_le_U32s = array_to_le_uint32s
 
+class array_assign (o: Type0) = {
+  key: Type0;
+  value: Type0;
+  (.[]<-): o -> key -> value -> o
+}
+
+instance array_upd1: array_assign state_t = {
+  key = state_idx;
+  value = uint32;
+  (.[]<-) = array_upd
+}
+
+instance array_upd2: array_assign constants_t = {
+  key = constants_idx;
+  value = uint32;
+  (.[]<-) = array_upd
+}
+class has_default (o: Type) = {new_: o}
+instance _: has_default state_t = {new_ = array_new_ (secret 0x0ul) 16}
+instance _: has_default constants_t = {new_ = array_new_ (secret 0x0ul) 4}
+instance _: has_default block_t = {new_ = array_new_ (secret (pub_u8 0x0)) 64}
 
 class xor (t: Type) = { (^.): t -> t -> t }
 instance xor_inherit t l: xor (int_t t l) = { (^.) = logxor }
@@ -65,6 +82,9 @@ instance add_lseq (len: uint_size) (t:Type) {| add t |}: add (lseq t len)
   = { (+.) = array_add (+.) }
 
 let slice = array_slice
+
+
+
 
 // class foldi_tc (key: eqtype) = {
 //   foldi_lt_key: key -> key -> bool;
