thir-elab/out/Hacspec_chacha20.fst
@@ -1,12 +1,43 @@
 module Hacspec_chacha20
+#set-options "--fuel 0 --ifuel 1 --z3rlimit 15"
+open FStar.Mul
+open Hacspec.Lib
+open Hacspec_lib_tc
 
-let chacha20_line (a b d s: uint_size) (m: state_t) : state_t =
+
+
+
+
+
+
+unfold
+type state_t = lseq uint32 16
+unfold
+type state_idx_t = nat_mod 16
+
+unfold
+type constants_t = lseq uint32 4
+unfold
+type constants_idx_t = nat_mod 4
+
+unfold
+type block_t = lseq uint8 64
+
+unfold
+type chaChaIV_t = lseq uint8 12
+
+unfold
+type chaChaKey_t = lseq uint8 32
+
+let chacha20_line (a b d: state_idx_t) (s: pos {s < 32}) (m: state_t) : state_t =
   let state:state_t = m in
   let state:state_t = state.[ a ] <- state.[ a ] +. state.[ b ] in
   let state:state_t = state.[ d ] <- state.[ d ] ^. state.[ a ] in
   state.[ d ] <- Secret_integers.rotate_left state.[ d ] s
 
-let chacha20_quarter_round (a b c d: uint_size) (state: state_t) : state_t =
+
+
+let chacha20_quarter_round (a b c d: state_idx_t) (state: state_t) : state_t =
   let state:state_t = chacha20_line a b d 16 state in
   let state:state_t = chacha20_line c d b 12 state in
   let state:state_t = chacha20_line a b d 8 state in
@@ -24,12 +55,9 @@ let chacha20_double_round (state: state_t) : state_t =
 
 let chacha20_rounds (state: state_t) : state_t =
   let st:state_t = state in
-  let _:Prims.unit =
-    Dummy.foldi 0 10 (fun (i: uint_size) (st: state_t) -> chacha20_double_round st) st
-  in
-  st
+  foldi 0 10 (fun (_i: uint_size) (st: state_t) -> chacha20_double_round st) st
 
-let chacha20_core (ctr: Hacspec_lib.secret_t) (st0: state_t) : state_t =
+let chacha20_core (ctr: Secret_integers.u32_t) (st0: state_t) : state_t =
   let state:state_t = st0 in
   let state:state_t = state.[ 12 ] <- state.[ 12 ] +. ctr in
   let k:state_t = chacha20_rounds state in
@@ -37,27 +65,27 @@ let chacha20_core (ctr: Hacspec_lib.secret_t) (st0: state_t) : state_t =
 
 let chacha20_constants_init: constants_t =
   let constants:constants_t = new_ in
-  let constants:constants_t = constants.[ 0 ] <- Hacspec_lib.secret 1634760805ul in
-  let constants:constants_t = constants.[ 1 ] <- Hacspec_lib.secret 857760878ul in
-  let constants:constants_t = constants.[ 2 ] <- Hacspec_lib.secret 2036477234ul in
-  constants.[ 3 ] <- Hacspec_lib.secret 1797285236ul
+  let constants:constants_t = constants.[ 0 ] <- Hacspec_lib_tc.secret 1634760805ul in
+  let constants:constants_t = constants.[ 1 ] <- Hacspec_lib_tc.secret 857760878ul in
+  let constants:constants_t = constants.[ 2 ] <- Hacspec_lib_tc.secret 2036477234ul in
+  constants.[ 3 ] <- Hacspec_lib_tc.secret 1797285236ul
 
-let chacha20_init (key: chaChaKey_t) (iv: chaChaIV_t) (ctr: Hacspec_lib.secret_t) : state_t =
+let chacha20_init (key: chaChaKey_t) (iv: chaChaIV_t) (ctr: Secret_integers.u32_t) : state_t =
   let st:state_t = new_ in
-  let st:state_t = Hacspec_lib.update st 0 chacha20_constants_init in
-  let st:state_t = Hacspec_lib.update st 4 (to_le_U32s key) in
+  let st:state_t = Hacspec_lib_tc.update st 0 chacha20_constants_init in
+  let st:state_t = Hacspec_lib_tc.update st 4 (to_le_U32s key) in
   let st:state_t = st.[ 12 ] <- ctr in
-  Hacspec_lib.update st 13 (to_le_U32s iv)
+  Hacspec_lib_tc.update st 13 (to_le_U32s iv)
 
 let chacha20_key_block (state: state_t) : block_t =
-  let state:state_t = chacha20_core (Hacspec_lib.secret 0ul) state in
+  let state:state_t = chacha20_core (Hacspec_lib_tc.secret 0ul) state in
   from_seq (to_le_bytes state)
 
 let chacha20_key_block0 (key: chaChaKey_t) (iv: chaChaIV_t) : block_t =
-  let state:state_t = chacha20_init key iv (Hacspec_lib.secret 0ul) in
+  let state:state_t = chacha20_init key iv (Hacspec_lib_tc.secret 0ul) in
   chacha20_key_block state
 
-let chacha20_encrypt_block (st0: state_t) (ctr: Hacspec_lib.secret_t) (plain: block_t) : block_t =
+let chacha20_encrypt_block (st0: state_t) (ctr: Secret_integers.u32_t) (plain: block_t) : block_t =
   let st:state_t = chacha20_core ctr st0 in
   let pl:state_t = from_seq (to_le_U32s plain) in
   let st:state_t = pl ^. st in
@@ -65,45 +93,49 @@ let chacha20_encrypt_block (st0: state_t) (ctr: Hacspec_lib.secret_t) (plain: bl
 
 let chacha20_encrypt_last
       (st0: state_t)
-      (ctr: Hacspec_lib.secret_t)
-      (plain: Hacspec_lib.seq_t Secret_integers.u8_t)
-    : Hacspec_lib.seq_t Secret_integers.u8_t =
+      (ctr: Secret_integers.u32_t)
+      (plain: Hacspec_lib_tc.seq_t Secret_integers.u8_t {seq_len plain < 64})
+    : Hacspec_lib_tc.seq_t Secret_integers.u8_t =
   let b:block_t = new_ in
-  let b:block_t = Hacspec_lib.update b 0 plain in
+  let b:block_t = Hacspec_lib_tc.update b 0 plain in
   let b:block_t = chacha20_encrypt_block st0 ctr b in
-  slice b 0 (Hacspec_lib.len plain)
+  slice b 0 (Hacspec_lib_tc.len plain)
 
-let chacha20_update (st0: state_t) (m: Hacspec_lib.seq_t Secret_integers.u8_t)
-    : Hacspec_lib.seq_t Secret_integers.u8_t =
-  let blocks_out:Hacspec_lib.seq_t Secret_integers.u8_t = Hacspec_lib.new_ (Hacspec_lib.len m) in
-  let n_blocks:uint_size = Hacspec_lib.num_exact_chunks m 64 in
-  let _:Prims.unit =
-    Dummy.foldi 0
+let chacha20_update (st0: state_t) (m: Hacspec_lib_tc.seq_t Secret_integers.u8_t)
+    : Hacspec_lib_tc.seq_t Secret_integers.u8_t =
+  let blocks_out =
+    Hacspec_lib_tc.new_seq (Hacspec_lib_tc.len m)
+  in
+  let n_blocks:uint_size = Hacspec_lib_tc.num_exact_chunks m 64 in
+  let blocks_out =
+    foldi 0
       n_blocks
-      (fun (i: uint_size) (blocks_out: Hacspec_lib.seq_t Secret_integers.u8_t) ->
-          let msg_block:Hacspec_lib.seq_t Secret_integers.u8_t =
-            Hacspec_lib.get_exact_chunk m 64 i
+      (fun i blocks_out ->
+          let msg_block:Hacspec_lib_tc.seq_t Secret_integers.u8_t =
+            Hacspec_lib_tc.get_exact_chunk m 64 i
           in
-          let b:block_t = chacha20_encrypt_block st0 (Hacspec_lib.secret i) (from_seq msg_block) in
-          Hacspec_lib.set_exact_chunk blocks_out 64 i b)
+          let b:block_t =
+            chacha20_encrypt_block st0 (Hacspec_lib_tc.secret i) (from_seq msg_block)
+          in
+          Hacspec_lib_tc.set_exact_chunk blocks_out 64 i b)
       blocks_out
   in
-  let last_block:Hacspec_lib.seq_t Secret_integers.u8_t = Hacspec_lib.get_remainder_chunk m 64 in
-  let _, blocks_out:(Prims.unit * Hacspec_lib.seq_t Secret_integers.u8_t) =
-    if Hacspec_lib.len last_block <> 0
-    then
-      let b:Hacspec_lib.seq_t Secret_integers.u8_t =
-        chacha20_encrypt_last st0 (Hacspec_lib.secret n_blocks) last_block
-      in
-      Hacspec_lib.set_chunk blocks_out 64 n_blocks b
+  let last_block:Hacspec_lib_tc.seq_t Secret_integers.u8_t =
+    Hacspec_lib_tc.get_remainder_chunk m 64
   in
-  blocks_out
+  if Hacspec_lib_tc.len last_block <> 0
+  then
+    let b:Hacspec_lib_tc.seq_t Secret_integers.u8_t =
+      chacha20_encrypt_last st0 (Hacspec_lib_tc.secret n_blocks) last_block
+    in
+    Hacspec_lib_tc.set_chunk blocks_out 64 n_blocks b
+  else blocks_out
 
 let chacha20
       (key: chaChaKey_t)
       (iv: chaChaIV_t)
       (ctr: UInt32.t)
-      (m: Hacspec_lib.seq_t Secret_integers.u8_t)
-    : Hacspec_lib.seq_t Secret_integers.u8_t =
-  let state:state_t = chacha20_init key iv (Hacspec_lib.secret ctr) in
+      (m: Hacspec_lib_tc.seq_t Secret_integers.u8_t)
+    : Hacspec_lib_tc.seq_t Secret_integers.u8_t =
+  let state:state_t = chacha20_init key iv (Hacspec_lib_tc.secret ctr) in
   chacha20_update state m
