thir-elab/Hacspec_lib.fst
@@ -1,0 +1,4 @@
+module Hacspec_lib
+open Hacspec.Lib
+
+
