thir-elab/out/Example.fst
@@ -1,0 +1,6 @@
+module Example
+
+let test: UInt8.t =
+  let acc:UInt8.t = 0uy in
+  let acc:UInt8.t = Dummy.foldi 1uy 10uy (fun (i: UInt8.t) (acc: UInt8.t) -> acc + i) acc in
+  acc + 1uy
