thir-elab/out/Hacspec_poly1305.Edited.fst
@@ -1,0 +1,114 @@
+module Hacspec_poly1305
+#set-options "--fuel 0 --ifuel 1 --z3rlimit 15"
+open FStar.Mul
+open Hacspec.Lib
+open Hacspec_lib_tc
+
+unfold
+type polyKey_t = lseq uint8 32
+
+let bLOCKSIZE: uint_size = 16
+
+unfold
+type polyBlock_t = lseq uint8 16
+
+unfold
+type poly1305Tag_t = lseq uint8 16
+
+let subBlock = Hacspec_lib_tc.seq_t Secret_integers.u8_t
+
+let blockIndex = uint_size
+
+unfold
+type fieldElement_t = nat_mod 0x03fffffffffffffffffffffffffffffffb
+unfold
+type fieldCanvas_t = lseq pub_uint8 131
+
+let polyState = (fieldElement_t & fieldElement_t & polyKey_t)
+
+unfold type sub_block_t = s: byte_seq {seq_len s < 16}
+type block_index_t = x: uint_size {x < bLOCKSIZE}
+
+let poly1305_encode_r (huhub: polyBlock_t) : fieldElement_t =
+  let n:Secret_integers.u128_t =
+    Hacspec_lib_tc.uint128_from_le_bytes (Hacspec_lib_tc.from_seq huhub)
+  in
+  let n = n &. Hacspec_lib_tc.secret (pub_u128 21267647620597763993911028882763415551) in
+  from_secret_literal n
+
+let poly1305_encode_block (xxb: polyBlock_t) : fieldElement_t =
+  let n:Secret_integers.u128_t =
+    Hacspec_lib_tc.uint128_from_le_bytes (Hacspec_lib_tc.from_seq xxb)
+  in
+  let f:fieldElement_t = from_secret_literal n in
+  f +. pow2 128
+
+let poly1305_encode_last (pad_len: block_index_t) (b: sub_block_t)
+    : fieldElement_t =
+  let n:Secret_integers.u128_t =
+    Hacspec_lib_tc.uint128_from_le_bytes (Hacspec_lib_tc.from_slice b 0 (Hacspec_lib_tc.len b))
+  in
+  let f:fieldElement_t = from_secret_literal n in
+  assert_norm (0x03fffffffffffffffffffffffffffffffb > pow2 129);
+  Math.Lemmas.pow2_lt_compat 129 (8 * pad_len);
+  f +. pow2 (8 * pad_len)
+
+let poly1305_init (k: polyKey_t) : (fieldElement_t & fieldElement_t & polyKey_t) =
+  let r:fieldElement_t = poly1305_encode_r (from_slice k 0 16) in
+  Hacspec_lib_tc.zero, r, k
+
+let poly1305_update_block (b: polyBlock_t) (st: (fieldElement_t & fieldElement_t & polyKey_t))
+    : (fieldElement_t & fieldElement_t & polyKey_t) =
+  let acc, r, k:(fieldElement_t & fieldElement_t & polyKey_t) = st in
+  (poly1305_encode_block b +. acc) *. r, r, k
+
+let poly1305_update_blocks
+      (m: Hacspec_lib_tc.seq_t Secret_integers.u8_t)
+      (st: (fieldElement_t & fieldElement_t & polyKey_t))
+    : (fieldElement_t & fieldElement_t & polyKey_t) =
+  let st:(fieldElement_t & fieldElement_t & polyKey_t) = st in
+  let n_blocks:uint_size = Prims.op_Division (Hacspec_lib_tc.len m) bLOCKSIZE in
+  Hacspec.Lib.foldi 0
+    n_blocks
+    (fun i st ->
+        let block:polyBlock_t = from_seq (Hacspec_lib_tc.get_exact_chunk m bLOCKSIZE i) in
+        poly1305_update_block block st)
+    st
+
+let poly1305_update_last
+      (pad_len: block_index_t)
+      (b: sub_block_t)
+      (st: (fieldElement_t & fieldElement_t & polyKey_t))
+    : (fieldElement_t & fieldElement_t & polyKey_t) =
+  let st:(fieldElement_t & fieldElement_t & polyKey_t) = st in
+  if Hacspec_lib_tc.len b <> 0
+  then
+    let acc, r, k:(fieldElement_t & fieldElement_t & polyKey_t) = st in
+    (poly1305_encode_last pad_len b +. acc) *. r, r, k
+  else st
+
+let poly1305_update
+      (m: Hacspec_lib_tc.seq_t Secret_integers.u8_t)
+      (st: (fieldElement_t & fieldElement_t & polyKey_t))
+    : (fieldElement_t & fieldElement_t & polyKey_t) =
+  let st:(fieldElement_t & fieldElement_t & polyKey_t) = poly1305_update_blocks m st in
+  let last:Hacspec_lib_tc.seq_t Secret_integers.u8_t =
+    Hacspec_lib_tc.get_remainder_chunk m bLOCKSIZE
+  in
+  poly1305_update_last (Hacspec_lib_tc.len last) last st
+
+let poly1305_finish (st: (fieldElement_t & fieldElement_t & polyKey_t)) : poly1305Tag_t =
+  let acc, _, k:(fieldElement_t & fieldElement_t & polyKey_t) = st in
+  let n:Secret_integers.u128_t =
+    Hacspec_lib_tc.uint128_from_le_bytes (Hacspec_lib_tc.from_slice k 16 16)
+  in
+  let aby:Hacspec_lib_tc.seq_t Secret_integers.u8_t = nat_to_byte_seq_le (0x03fffffffffffffffffffffffffffffffb) (17) acc in
+  let a:Secret_integers.u128_t =
+    Hacspec_lib_tc.uint128_from_le_bytes (Hacspec_lib_tc.from_slice aby 0 16)
+  in
+  from_seq (Hacspec_lib_tc.u128_to_le_bytes (a +. n))
+
+let poly1305 (m: Hacspec_lib_tc.seq_t Secret_integers.u8_t) (key: polyKey_t) : poly1305Tag_t =
+  let st:(fieldElement_t & fieldElement_t & polyKey_t) = poly1305_init key in
+  let st:(fieldElement_t & fieldElement_t & polyKey_t) = poly1305_update m st in
+  poly1305_finish st
