thir-elab/out/Secret_integers.fst
@@ -8,3 +8,15 @@ let rotate_left (u: uint32) (s: int{s > 0 /\ s < 32}) : uint32
 unfold type secret_t = uint32
 
 unfold type u8_t = uint8
+unfold type u16_t = uint16
+unfold type u32_t = uint32
+unfold type u64_t = uint64
+unfold type u128_t = uint128
+
+unfold let u8 x = Hacspec.Lib.secret #U8 (pub_u8 x)
+unfold let u16 x = Hacspec.Lib.secret #U16 (pub_u16 x)
+unfold let u32 x = Hacspec.Lib.secret #U32 (pub_u32 x)
+unfold let u64 x = Hacspec.Lib.secret #U64 (pub_u64 x)
+unfold let u128 x = Hacspec.Lib.secret #U128 (pub_u128 x)
+
+
